src/tlogic/SimWeakest.v
@@ -1985,27 +1985,28 @@ Section TRIPLES.
   (** LAT. *)
 
   Definition LAT_ind
-             n m
-             tid (P : iProp) {RV} (Q : RV -> iProp) (E : coPset)
-             {R_term : Type}
-             ps pt
-             (itr_src : itree srcE R_term) (code : itree tgtE RV) (ktr_tgt : ktree tgtE RV R_term)
+             tid n (E : coPset)
+             (P : iProp) {RV} (code : itree tgtE RV) (Q : RV -> iProp)
     : iProp
     :=
-    ((=|n|={E, ∅}=>
+    (∀ R_term ps pt
+       (itr_src : itree srcE R_term)
+       (ktr_tgt : RV -> itree tgtE R_term),
+      (=|S n|={E, ∅}=>
         ((P)
            ∗
            (∀ (rv : RV),
                (Q rv)
                  -∗
-                 =|n|={∅, E}=> wpsim n tid ⊤ ibot7 ibot7 (@term_cond m tid R_term) ps true itr_src (ktr_tgt rv))))
+                 =|S n|={∅, E}=> wpsim (S n) tid ⊤ ibot7 ibot7 (@term_cond n tid R_term) ps true itr_src (ktr_tgt rv))))
        -∗
-       wpsim n tid ⊤ ibot7 ibot7 (@term_cond m tid R_term) ps pt itr_src (code >>= ktr_tgt))%I.
+       wpsim (S n) tid ⊤ ibot7 ibot7 (@term_cond n tid R_term) ps pt itr_src (code >>= ktr_tgt))%I.
 
 End TRIPLES.
 
 (** For triples. *)
 Ltac iStartTriple := iIntros (? ? ? ? ? ? ?).
+Ltac iStartLAT := iIntros (? ? ? ? ?).
 
 Notation "'[@' tid , n , E '@]' { P } code { v , Q }" :=
   (atomic_triple tid n E P code (fun v => Q))
@@ -2016,6 +2017,11 @@ Notation "'[@' tid , n , E '@]' ⧼ P ⧽ code ⧼ v , Q ⧽" :=
   (non_atomic_triple tid n E P code (fun v => Q))
     (at level 200, tid, n, E, P, code, v, Q at level 1,
       format "[@  tid ,  n ,  E  @] ⧼ P ⧽  code  ⧼ v ,  Q ⧽") : bi_scope.
+
+Notation "'{@' tid , n , E '@}' ⧼ P ⧽ code ⧼ v , Q ⧽" :=
+  (LAT_ind tid n E P code (fun v => Q))
+    (at level 200, tid, n, E, P, code, v, Q at level 1,
+      format "{@  tid ,  n ,  E  @} ⧼ P ⧽  code  ⧼ v ,  Q ⧽") : bi_scope.
 
 (** Simulation tactics. *)
 
